WIP

investigations/cava2/Sha256Properties.v
@@ -32,13 +32,13 @@ Require HmacSpec.SHA256.
 Import ListNotations.
 
 (* TODO: move to a more general file *)
-Lemma step_vec_as_tuple_cons {t n} x0 (xs : list (denote_type t)) :
-  step (vec_as_tuple (t:=t) (n:=S n)) tt (x0 :: xs, tt)
-  = (tt, (x0, snd (step (vec_as_tuple (t:=t) (n:=n)) tt (xs, tt)))).
+Lemma step_vec_as_tuple_cons {t n} (xs : list (denote_type t)) :
+  step (vec_as_tuple (t:=t) (n:=S n)) tt (xs, tt)
+  = (tt, (hd default xs, snd (step (vec_as_tuple (t:=t) (n:=n)) tt (tl xs, tt)))).
 Proof. reflexivity. Qed.
 Hint Rewrite @step_vec_as_tuple_cons using solve [eauto] : stepsimpl.
-Lemma step_vec_as_tuple_one {t} (x : denote_type t):
-  step (vec_as_tuple (t:=t) (n:=0)) tt ([x], tt) = (tt, x).
+Lemma step_vec_as_tuple_one {t} (xs : list (denote_type t)):
+  step (vec_as_tuple (t:=t) (n:=0)) tt (xs, tt) = (tt, hd default xs).
 Proof. reflexivity. Qed.
 Hint Rewrite @step_vec_as_tuple_one using solve [eauto] : stepsimpl.
 Ltac stepsimpl :=
@@ -64,17 +64,52 @@ Proof.
 Qed.
 Hint Rewrite @step_rotr using solve [eauto] : stepsimpl.
 
+(* TODO: move *)
+Lemma resize_length {A} (d : A) n ls : length (List.resize d n ls) = n.
+Proof. cbv [List.resize]. length_hammer. Qed.
+Hint Rewrite @resize_length using solve [eauto] : push_length.
+
+(* TODO: move *)
+Lemma firstn_map_nth {A} (d : A) n ls :
+  n <= length ls -> firstn n ls = List.map (fun i : nat => nth i ls d) (seq 0 n).
+Proof.
+  revert ls; induction n; [ reflexivity | ].
+  intros. erewrite firstn_succ_snoc by lia. rewrite IHn by lia.
+  autorewrite with pull_snoc. reflexivity.
+Qed.
+
+(* TODO: move *)
+Lemma resize_map_nth {A} (d : A) n ls :
+  List.resize d n ls = List.map (fun i => nth i ls d) (seq 0 n).
+Proof.
+  intros; subst. cbv [List.resize].
+  destr (n <=? length ls);
+    autorewrite with natsimpl listsimpl push_firstn;
+    [ solve [auto using firstn_map_nth] | ].
+  replace n with (length ls + (n - length ls)) by lia.
+  rewrite seq_app, map_app, <-firstn_map_nth by lia.
+  autorewrite with natsimpl push_firstn. apply f_equal.
+  erewrite map_ext_in; [ rewrite map_constant; f_equal; length_hammer | ].
+  intros *. rewrite in_seq. intros.
+  rewrite nth_overflow by lia; reflexivity.
+Qed.
+
+Lemma hd_to_nth {A} (d : A) ls : hd d ls = nth 0 ls d.
+Proof. destruct ls; reflexivity. Qed.
+Hint Rewrite @hd_to_nth @nth_tl using solve [eauto] : hd_tl_to_nth.
+
 Lemma step_sha256_compress
       (H : denote_type sha_digest)
       (k w : denote_type sha_word) (t i : nat) (msg : list byte) :
-  length H = 8 ->
   k = nth t SHA256.K 0%N ->
   w = nth t (SHA256.W msg i) 0%N ->
   step sha256_compress tt (H,(k,(w,tt)))
-  = (tt, SHA256.sha256_compress msg i H t).
+  = (tt, SHA256.sha256_compress msg i (List.resize 0%N 8 H) t).
 Proof.
-  intros. subst; destruct_lists_by_length.
-  cbv [sha256_compress]. stepsimpl. reflexivity.
+  intros. rewrite resize_map_nth. cbn [List.map seq].
+  subst. cbv [sha256_compress]. stepsimpl.
+  autorewrite with hd_tl_to_nth.
+  reflexivity.
 Qed.
 Hint Rewrite @step_sha256_compress using solve [eauto] : stepsimpl.
 
@@ -136,7 +171,7 @@ Lemma step_sha256_message_schedule_update
 Proof.
   intros. cbv [sha256_message_schedule_update]. stepsimpl.
   rewrite nth_W by lia. destruct_one_match; [ lia | ].
-  repeat match goal with H : _ = nth _ _ _ |- _ =>
+  repeat match goal with H : _ = nth ?n _ _ |- _ =>
                          rewrite <-H end.
   cbv [SHA256.add_mod SHA256.w]. N.push_pull_mod.
   cbv [SHA256.sigma1 SHA256.sigma0 SHA256.SHR].
@@ -145,8 +180,161 @@ Proof.
 Qed.
 Hint Rewrite @step_sha256_message_schedule_update using solve [eauto] : stepsimpl.
 
+(* TODO: move *)
+Lemma resize_noop {A} (d : A) n ls :
+  n = length ls -> List.resize d n ls = ls.
+Proof.
+  intros; subst. cbv [List.resize].
+  autorewrite with natsimpl listsimpl push_firstn.
+  reflexivity.
+Qed.
+
 Lemma step_sha256_round_constants (round : denote_type sha_round) :
   step sha256_round_constants tt (round, tt)
   = (tt, nth (N.to_nat round) SHA256.K 0%N).
 Proof. reflexivity. Qed.
 Hint Rewrite @step_sha256_round_constants using solve [eauto] : stepsimpl.
+
+Definition sha256_inner_spec
+           (input : denote_type [Bit; sha_block; sha_digest; Bit])
+           (state : denote_type (sha_digest ** sha_block ** Bit ** sha_round))
+           msg (i : nat)
+  : denote_type (sha_digest ** sha_block ** Bit ** sha_round)
+    * denote_type (sha_digest ** Bit) :=
+  let '(block_valid, (block, (initial_digest, clear))) := input in
+  let '(current_digest, (message_schedule, (done, round))) := state in
+  let inc_round := (done =? 0)%N in
+  let start := negb (block_valid =? 0)%N in
+  let t := N.to_nat round in
+  let next_message_schedule :=
+      List.resize 0%N 16 (firstn 16 (skipn (t + 1 - 16) (SHA256.W msg i))) in
+  let next_digest := SHA256.sha256_compress msg i current_digest t in
+  let next_done := if ((round =? 64)%N || negb (done =? 0)%N)%bool then 1%N else 0%N in
+  let next_round := if inc_round then (round + 1)%N else round in
+  let next_state := (next_digest, (next_message_schedule, (next_done, next_round))) in
+  let out := (map2 N.add initial_digest next_digest, next_done) in
+  (next_state, out).
+
+Definition state_of {s i o} (c : @Circuit denote_type s i o) : type := s.
+Compute state_of sha256_inner.
+
+(* TODO: move *)
+Module List.
+  Definition slice {A} (d : A) ls start len : list A :=
+    List.resize d len (skipn start ls).
+End List.
+
+Lemma nth_skipn {A} (d : A) n i ls :
+  nth i (skipn n ls) d = nth (n + i) ls d.
+Proof.
+  revert i ls; induction n; [ reflexivity | ].
+  intros; destruct ls; [ destruct i; reflexivity | ].
+  cbn [Nat.add]. autorewrite with push_skipn push_nth.
+  rewrite IHn. reflexivity.
+Qed.
+Hint Rewrite @nth_skipn using solve [eauto] : push_nth.
+
+(* TODO: move *)
+Lemma slice_map_nth {A} (d : A) ls start len :
+  List.slice d ls start len = List.map (fun i => nth (start + i) ls d) (seq 0 len).
+Proof.
+  intros; subst. cbv [List.slice].
+  rewrite resize_map_nth. apply map_ext; intros.
+  autorewrite with push_nth; reflexivity.
+Qed.
+
+(* TODO: move *)
+Lemma slice_length {A} (d : A) ls start len :
+  length (List.slice d ls start len) = len.
+Proof. rewrite slice_map_nth. length_hammer. Qed.
+Hint Rewrite @slice_length using solve [eauto] : push_length.
+
+(* TODO: move *)
+Lemma tl_slice {A} (d : A) ls start len :
+  tl (List.slice d ls start (S len)) = List.slice d ls (S start) len.
+Proof.
+  rewrite !slice_map_nth. cbn [seq List.map tl].
+  rewrite <-seq_shift, map_map. apply map_ext; intros.
+  f_equal; lia.
+Qed.
+
+(* TODO: move *)
+Lemma hd_slice {A} (d : A) ls start len :
+  hd d (List.slice d ls start (S len)) = nth start ls d.
+Proof.
+  rewrite !slice_map_nth. cbn [seq List.map hd]. f_equal; lia.
+Qed.
+
+Ltac is_projection_from_step e :=
+  lazymatch e with
+  | fst ?e' => is_projection_from_step e'
+  | snd ?e' => is_projection_from_step e'
+  | step _ _ _ => idtac
+  | _ => fail "term is not a projection from step"
+  end.
+
+(* works like destruct_pair_let, but only simplifies expressions with step *)
+Ltac destruct_step_pair_let :=
+  repeat match goal with
+         | |- context [match ?p with
+                      | pair _ _ => _ end] =>
+           is_projection_from_step p;
+           rewrite (surjective_pairing p)
+         end.
+
+Print SHA256.sha256_step.
+Lemma step_sha256_inner
+      (input : denote_type [Bit; sha_block; sha_digest; Bit])
+      (state : denote_type (sha_digest ** sha_block ** Bit ** sha_round))
+      msg i :
+  (* message schedule = 16 elts of W starting at index round-16 (0 if round <= 16) *)
+  fst (snd state) = List.slice 0%N (SHA256.W msg i)
+                               (N.to_nat (snd (snd (snd state))) - 16) 16 ->
+  step sha256_inner state input = sha256_inner_spec input state msg i.
+Proof.
+  Set Printing Depth 10000.
+  destruct input as (block_valid, (block, (initial_digest, (clear, [])))).
+  destruct state as (current_digest, (message_schedule, (done, round))).
+  cbn [fst snd]. intros; subst.
+  cbv [sha256_inner K]. stepsimpl.
+  destruct_step_pair_let. cbn [fst snd].
+  rewrite !resize_noop by length_hammer.
+  rewrite !tl_slice. rewrite !hd_slice.
+  erewrite step_sha256_compress with (t:=N.to_nat round).
+  2:{ reflexivity. }
+  2:{
+  rewrite slice_map_nth. cbn [List.map seq hd tl app].
+  rewrite !resize_noop by length_hammer. cbn [tl].
+  stepsimpl. destruct_step_pair_let.
+  cbn [tl].
+  destruct_pair_let; cbn [fst snd].
+  destruct_pair_let; cbn [fst snd].
+  destruct_pair_let; cbn [fst snd].
+  destruct_pair_let; cbn [fst snd].
+  destruct_pair_let; cbn [fst snd].
+  destruct_pair_let; cbn [fst snd].
+  destruct_pair_let; cbn [fst snd].
+  destr (15 <=? round)%N.
+  { cbn [N.eqb].
+    rewrite (surjective_pairing (step sha256_message_schedule_update _ _)).
+  erewrite step_sha256_message_schedule_update with (t:=N.to_nat round).
+  2:{ f_equal; lia. }
+  2:{ f_equal; try lia. }
+  2:{ f_equal; lia. }
+    rewrite firstn_
+  { erewrite step_sha256_compress.
+  rewrite step_sha256_round_constants.
+  intros. subst; destruct_lists_by_length.
+  cbv [sha256_compress]. stepsimpl. reflexivity.
+  intro Hschedule. rewrite resize_map_nth in Hschedule.
+  cbn [seq List.map] in Hschedule. subst.
+  cbv [sha256_inner K]. stepsimpl.
+  2:{
+    Search nth firstn.
+    rewrite firstn_
+  { erewrite step_sha256_compress.
+  rewrite step_sha256_round_constants.
+  intros. subst; destruct_lists_by_length.
+  cbv [sha256_compress]. stepsimpl. reflexivity.
+Qed.
+Hint Rewrite @step_sha256_compress using solve [eauto] : stepsimpl.
